ulib/experimental/Steel.SelHigherReference.fsti
@@ -1,0 +1,161 @@
+(*
+   Copyright 2020 Microsoft Research
+
+   Licensed under the Apache License, Version 2.0 (the "License");
+   you may not use this file except in compliance with the License.
+   You may obtain a copy of the License at
+
+       http://www.apache.org/licenses/LICENSE-2.0
+
+   Unless required by applicable law or agreed to in writing, software
+   distributed under the License is distributed on an "AS IS" BASIS,
+   WITHOUT WARRANTIES OR CONDITIONS OF ANY KIND, either express or implied.
+   See the License for the specific language governing permissions and
+   limitations under the License.o
+*)
+
+module Steel.SelHigherReference
+
+open Steel.FractionalPermission
+open FStar.Ghost
+
+open Steel.Memory
+open Steel.SelEffect.Atomic
+open Steel.SelEffect
+
+module Mem = Steel.Memory
+
+val ref (a:Type u#1) : Type u#0
+
+val null (#a:Type u#1) : ref a
+val is_null (#a:Type u#1) (r:ref a) : (b:bool{b <==> r == null})
+
+val pts_to_sl (#a:Type u#1) (r:ref a) (p:perm) (v:erased a) : slprop u#1
+
+[@@ __steel_reduce__]
+unfold let pts_to (#a:Type u#1) (r:ref a) (p:perm) (v:erased a) : vprop =
+  to_vprop (pts_to_sl r p v)
+
+val pts_to_ref_injective
+      (#a: Type u#1)
+      (r: ref a)
+      (p0 p1:perm)
+      (v0 v1: erased a)
+      (m:mem)
+    : Lemma
+      (requires
+        interp (pts_to_sl r p0 v0 `Mem.star` pts_to_sl r p1 v1) m)
+      (ensures v0 == v1)
+
+val pts_to_not_null (#a:Type u#1)
+                    (x:ref a)
+                    (p:perm)
+                    (v: erased a)
+                    (m:mem)
+  : Lemma (requires interp (pts_to_sl x p v) m)
+          (ensures x =!= null)
+
+val pts_to_witinv (#a:Type) (r:ref a) (p:perm) : Lemma (is_witness_invariant (pts_to_sl r p))
+
+val higher_ref_pts_to_injective_eq
+      (#a: Type)
+      (#opened:inames)
+      (#p0 #p1:perm)
+      (#v0 #v1: erased a)
+      (r: ref a)
+  : SteelSelGhost unit opened
+          (pts_to r p0 v0 `star` pts_to r p1 v1)
+          (fun _ -> pts_to r p0 v0 `star` pts_to r p1 v0)
+          (requires fun _ -> True)
+          (ensures fun _ _ _ -> v0 == v1)
+
+val alloc (#a:Type) (x:a)
+  : SteelSelT (ref a) emp (fun r -> pts_to r full_perm x)
+
+val read (#a:Type) (#p:perm) (#v:erased a) (r:ref a)
+  : SteelSel a (pts_to r p v) (fun x -> pts_to r p x)
+           (requires fun h -> True)
+           (ensures fun _ x _ -> x == Ghost.reveal v)
+
+val read_refine (#a:Type) (#p:perm) (q:a -> vprop) (r:ref a)
+  : SteelSelT a (h_exists (fun (v:a) -> pts_to r p v `star` q v))
+             (fun v -> pts_to r p v `star` q v)
+
+val write (#a:Type) (#v:erased a) (r:ref a) (x:a)
+  : SteelSelT unit (pts_to r full_perm v) (fun _ -> pts_to r full_perm x)
+
+val free (#a:Type) (#v:erased a) (r:ref a)
+  : SteelSelT unit (pts_to r full_perm v) (fun _ -> emp)
+
+val share (#a:Type) (#uses:_) (#p:perm) (#v:erased a) (r:ref a)
+  : SteelSelGhostT unit uses
+    (pts_to r p v)
+    (fun _ -> pts_to r (half_perm p) v `star` pts_to r (half_perm p) v)
+
+val gather (#a:Type) (#uses:_) (#p0:perm) (#p1:perm) (#v0 #v1:erased a) (r:ref a)
+  : SteelSelGhost unit uses
+    (pts_to r p0 v0 `star` pts_to r p1 v1)
+    (fun _ -> pts_to r (sum_perm p0 p1) v0)
+    (requires fun _ -> True)
+    (ensures fun _ _ _ -> v0 == v1)
+
+val cas_action (#t:Type) (eq: (x:t -> y:t -> b:bool{b <==> (x == y)}))
+               (#uses:inames)
+               (r:ref t)
+               (v:Ghost.erased t)
+               (v_old:t)
+               (v_new:t)
+   : action_except (b:bool{b <==> (Ghost.reveal v == v_old)})
+                   uses
+                   (pts_to_sl r full_perm v)
+                   (fun b -> if b then pts_to_sl r full_perm v_new else pts_to_sl r full_perm v)
+
+(*** Ghost references ***)
+
+[@@ erasable]
+val ghost_ref (a:Type u#1) : Type u#0
+
+val ghost_pts_to_sl (#a:_) (r:ghost_ref a) (p:perm) (x:erased a) : slprop u#1
+
+[@@ __steel_reduce__]
+unfold let ghost_pts_to (#a:_) (r:ghost_ref a) (p:perm) (x:erased a) : vprop =
+  to_vprop (ghost_pts_to_sl r p x)
+
+val ghost_pts_to_witinv (#a:Type) (r:ghost_ref a) (p:perm) : Lemma (is_witness_invariant (ghost_pts_to_sl r p))
+
+val ghost_alloc (#a:Type) (#u:_) (x:erased a)
+  : SteelSelGhostT (ghost_ref a) u
+                 emp
+                 (fun r -> ghost_pts_to r full_perm x)
+
+val ghost_share (#a:Type) (#u:_)
+                (#p:perm)
+                (#x:erased a)
+                (r:ghost_ref a)
+  : SteelSelGhostT unit u
+    (ghost_pts_to r p x)
+    (fun _ -> ghost_pts_to r (half_perm p) x `star`
+           ghost_pts_to r (half_perm p) x)
+
+val ghost_gather (#a:Type) (#u:_)
+                 (#p0 #p1:perm)
+                 (#x0 #x1:erased a)
+                 (r:ghost_ref a)
+  : SteelSelGhost unit u
+    (ghost_pts_to r p0 x0 `star`
+     ghost_pts_to r p1 x1)
+    (fun _ -> ghost_pts_to r (sum_perm p0 p1) x0)
+    (requires fun _ -> True)
+    (ensures fun _ _ _ -> x0 == x1)
+
+val ghost_pts_to_injective_eq (#a:_) (#u:_) (#p #q:_) (r:ghost_ref a) (v0 v1:Ghost.erased a)
+  : SteelSelGhost unit u
+    (ghost_pts_to r p v0 `star` ghost_pts_to r q v1)
+    (fun _ -> ghost_pts_to r p v0 `star` ghost_pts_to r q v0)
+    (requires fun _ -> True)
+    (ensures fun _ _ _ -> v0 == v1)
+
+val ghost_write (#a:Type) (#u:_) (#v:erased a) (r:ghost_ref a) (x:erased a)
+  : SteelSelGhostT unit u
+    (ghost_pts_to r full_perm v)
+    (fun _ -> ghost_pts_to r full_perm x)
